0.3 finished

cpdt_0.3.v
@@ -1,51 +1,94 @@
 Require Import Cpdt.CpdtTactics.
 
+Set Implicit Arguments.
+
 (* 1 *)
 CoInductive itree (A : Type) : Type :=
 | Node : A -> itree A -> itree A -> itree A.
 
 CoFixpoint everywhere {A : Type} (x : A) : itree A :=
-  Node A x (everywhere x) (everywhere x).
+  Node x (everywhere x) (everywhere x).
 
 CoFixpoint map {A B C : Type} (f : A -> B -> C)
     (t1 : itree A) (t2 : itree B) :=
-  match t1 with Node _ x l1 r1
-  => match t2 with Node _ y l2 r2
-      => Node _ (f x y) (map f l1 l2) (map f r1 r2)
-     end
+  match (t1, t2) with
+  | (Node x l1 r1, Node y l2 r2) =>
+      Node (f x y) (map f l1 l2) (map f r1 r2)
   end.
 
-CoFixpoint falses := everywhere true.
+CoFixpoint falses := everywhere false.
+CoFixpoint trues := everywhere true.
 
-CoFixpoint true_false : itree bool :=
-  Node bool true
-    (Node bool false true_false true_false)
-    (Node bool false true_false true_false).
+CoFixpoint true_false : itree bool := let ft := Node false true_false true_false in
+  Node true ft ft.
 
 CoFixpoint true_false' : itree bool :=
-  Node bool true false_true' false_true'
+  Node true false_true' false_true'
 with false_true' : itree bool :=
-  Node bool false true_false' true_false'.
+  Node false true_false' true_false'.
 
 CoInductive itree_eq {A : Type} : itree A -> itree A ->Prop :=
   | ITree_eq : forall x l1 l2 r1 r2, itree_eq l1 l2 -> itree_eq r1 r2 ->
-      itree_eq (Node _ x l1 r1) (Node _ x l2 r2).
+      itree_eq (Node x l1 r1) (Node x l2 r2).
 
-Definition useless {A : Type} (t : itree A) :=
+Definition u {A : Type} (t : itree A) :=
   match t with
-  | Node _ x l r => Node A x l r
+  | Node x l r => Node x l r
   end.
 
-Theorem useless_is_useful : forall {A : Type} (t : itree A), t = useless t.
+Theorem uiu : forall {A : Type} (t : itree A), t = u t.
 Proof.
   intros; destruct t; reflexivity.
 Qed.
 
+Definition value {A : Type} (t : itree A) : A :=
+  match t with
+  | Node x _ _ => x
+  end.
+
+Definition left {A : Type} (t : itree A) : itree A :=
+  match t with
+  | Node _ l _ => l
+  end.
+
+Definition right {A : Type} (t : itree A) : itree A :=
+  match t with
+  | Node _ _ r => r
+  end.
+
+Section itree_eq_coind.
+  Variable A : Type.
+  Variable R : itree A -> itree A -> Prop.
+
+  Hypothesis Value_case : forall t1 t2, R t1 t2 -> value t1 = value t2.
+  Hypothesis Left_case : forall t1 t2, R t1 t2 -> R (left t1) (left t2).
+  Hypothesis Right_case : forall t1 t2, R t1 t2 -> R (right t1) (right t2).
+
+  Theorem itree_eq_coind : forall t1 t2, R t1 t2 -> itree_eq t1 t2.
+  Proof.
+    cofix; destruct t1; destruct t2; intros.
+    generalize (Value_case H); intro; simpl in H0; rewrite <- H0.
+    constructor; apply itree_eq_coind; [ apply (Left_case H) | apply (Right_case H) ].
+  Qed.
+End itree_eq_coind.
+
 Require Import Bool.
+Check itree_eq_coind.
 
-Theorem true_false_or : itree_eq true_false (map orb true_false falses).
+Theorem false_is_fixp : forall b, b || false = b.
 Proof.
-  cofix. rewrite (useless_is_useful true_false).
-  rewrite (useless_is_useful (map _ _ _)). simpl.
+  destruct b; reflexivity.
+Qed.
 
+Hint Rewrite false_is_fixp.
+
+Theorem falses_is_fixp : forall t, itree_eq t (map orb t (everywhere false)).
+Proof.
+  cofix; destruct t; rewrite (uiu (map _ _ _)); crush;
+  constructor; apply falses_is_fixp.
+Qed.
+
+Theorem true_false_or : itree_eq true_false (map orb true_false (everywhere false)).
+Proof.
+  cofix; apply (falses_is_fixp true_false).
 Qed.
